Presheaf/Gpd: identify groupoid presentations with pseudofunctors

theories/Presheaf/FaceStructure.v
@@ -1,5 +1,6 @@
 (** Face maps on arbitrary type families indexed by dimension, with the
-    exchange law. No truncation of the levels is assumed. *)
+    exchange law and its hexagon coherence. No truncation of the levels is
+    assumed. *)
 
 Set Warnings "-notation-overridden".
 From Bonak.Lib Require Import HSet Notation LeSProp.
@@ -47,3 +48,27 @@ Definition topCoh {A: HSet} {Q: FaceStr A} (H: CohOf Q):
     sTop Q k ε (Q.(SFace) (S k) q (↑ Hq) ω X)
     = Q.(SFace) k q Hq ω (sTop Q (S k) ε X) :=
   fun k q Hq ε ω X => H k k leR_refl q Hq ε ω X.
+
+(** The hexagon coherence
+
+    [Coh2Of] equates the two three-step composites of exchange paths that
+    reorder three faces. The bounds [s <= r <= q] specify the indices before
+    the shifts introduced by each exchange. *)
+
+Definition Coh2Of {A: HSet} {Q: FaceStr A} (HQ: CohOf Q): Type :=
+  forall n q (Hq: q <= n) r (Hr: r <= q) s (Hs: s <= r) (ε ω θ: A)
+    (X: Q.(S0) (S (S (S n)))),
+    f_equal (Q.(SFace) n q Hq ε) (HQ (S n) r (Hr ↕ (↑ Hq)) s Hs ω θ X)
+    • (HQ n q Hq s (Hs ↕ Hr) ε θ
+         (Q.(SFace) (S (S n)) (S r) (⇑ (Hr ↕ (↑ Hq))) ω X)
+       • f_equal (Q.(SFace) n s (Hs ↕ (Hr ↕ Hq)) θ)
+           (HQ (S n) (S q) (⇑ Hq) (S r) (⇑ Hr) ε ω X))
+    = HQ n q Hq r Hr ε ω (Q.(SFace) (S (S n)) s (↑ (↑ (Hs ↕ (Hr ↕ Hq)))) θ X)
+      • (f_equal (Q.(SFace) n r (Hr ↕ Hq) ω)
+           (HQ (S n) (S q) (⇑ Hq) s (↑ (Hs ↕ Hr)) ε θ X)
+         • HQ n r (Hr ↕ Hq) s Hs ω θ
+             (Q.(SFace) (S (S n)) (S (S q)) (⇑ (⇑ Hq)) ε X)).
+
+Definition cohShift2 {A: HSet} {Q: FaceStr A} {HQ: CohOf Q} (H: Coh2Of HQ):
+  Coh2Of (cohShift HQ) :=
+  fun n q Hq r Hr s Hs ε ω θ X => H (S n) q (↑ Hq) r Hr s Hs ε ω θ X.
