theories/Presheaf/Gpd/Correspondence.v
@@ -1,0 +1,71 @@
+(** Groupoid-valued face presentations are equivalent to pseudofunctors
+    from the locally discrete opposite ν-semi-shape category to [HGpd2Cat].
+
+    The inverse translations restrict to generating cofaces and interpret
+    faces along words. [ofToPseudofunctor] and [toOfPseudofunctor] identify
+    their composites with the identity. The family of levels is preserved
+    definitionally in both directions. *)
+
+Set Warnings "-notation-overridden".
+From Bonak Require Import HSet Notation.
+
+From Bonak.Lib Require Import Equiv.
+From Bonak Require Import Univalence.
+
+From Bonak.Category Require Import Category.
+From Bonak.Category.Bicategory Require Import Bicategory LocallyDiscrete Pseudofunctor.
+From Bonak.Category Require Import Groupoid.
+From Bonak.Category.Bicategory Require Import PathGroupoid.
+From Bonak.Presheaf Require Import νSemiShape.
+From Bonak.Presheaf.Gpd Require Export Roundtrip.
+
+From Bonak.Category.Bicategory Require Import HGpd2Cat.
+From Bonak.Category.Bicategory Require Import UnivGpd2Cat.
+
+Set Primitive Projections.
+Set Printing Projections.
+
+Section CorrespondenceGpd.
+Context (A: HSet).
+
+Definition pshGpdEquivPsf:
+  Equiv (PresheafGpd A) (Pseudofunctor (locallyDiscrete (Op (νSemiShape A))) HGpd2Cat) :=
+  qinvEquiv (toPseudofunctor A) (ofPseudofunctor A)
+    (ofToPseudofunctor A) (toOfPseudofunctor A).
+
+End CorrespondenceGpd.
+
+(** The groupoid-level correspondence as an equality of types, by
+    univalence. *)
+
+Definition pshGpdEqPsf (A: HSet):
+  PresheafGpd A = Pseudofunctor (locallyDiscrete (Op (νSemiShape A))) HGpd2Cat :=
+  ua (pshGpdEquivPsf A).
+
+(** The same correspondence with the target read as the 2-category of
+    univalent groupoids, through the identification of the two targets. *)
+
+Definition pshGpdEqPsfGpd (A: HSet):
+  PresheafGpd A = Pseudofunctor (locallyDiscrete (Op (νSemiShape A))) UnivGpd2Cat :=
+  pshGpdEqPsf A
+  • f_equal (fun T: Bicategory => Pseudofunctor (locallyDiscrete (Op (νSemiShape A))) T) hgpd2CatEqUnivGpd2Cat.
+
+(** The augmented semi-simplicial and semi-cubical instances. *)
+
+Definition simplicialPresheafGpdEqPsf:
+  AugmentedSemiSimplicialPresheafGpd
+  = Pseudofunctor (locallyDiscrete (Op (νSemiShape hunit))) HGpd2Cat :=
+  pshGpdEqPsf hunit.
+
+Definition cubicalPresheafGpdEqPsf:
+  SemiCubicalPresheafGpd = Pseudofunctor (locallyDiscrete (Op (νSemiShape hbool))) HGpd2Cat :=
+  pshGpdEqPsf hbool.
+
+Definition simplicialPresheafGpdEqPsfGpd:
+  AugmentedSemiSimplicialPresheafGpd
+  = Pseudofunctor (locallyDiscrete (Op (νSemiShape hunit))) UnivGpd2Cat :=
+  pshGpdEqPsfGpd hunit.
+
+Definition cubicalPresheafGpdEqPsfGpd:
+  SemiCubicalPresheafGpd = Pseudofunctor (locallyDiscrete (Op (νSemiShape hbool))) UnivGpd2Cat :=
+  pshGpdEqPsfGpd hbool.
