theories/Presheaf/Gpd/Presentation.v
@@ -1,0 +1,121 @@
+(** Groupoid-valued presheaves presented by face maps and coherent
+    exchange paths, with an [HGpd] of cells at each level.
+
+    The exchange paths are data. [GFaceCoh2] identifies their two composites
+    around the hexagon for three deletions. Since identity types of an
+    [HGpd] are h-sets, any two proofs of this hexagon agree by [GUIP]. *)
+
+Set Warnings "-notation-overridden".
+From Bonak Require Import HSet Notation LeSProp νGpd.HGpd.
+
+From Bonak.Presheaf Require Import FaceStructure.
+
+From Bonak.Lib Require Import Funext.
+From Stdlib Require Import Logic.FunctionalExtensionality.
+
+Set Primitive Projections.
+Set Printing Projections.
+
+Record PresheafGpd (arity: HSet) := {
+  G0: nat -> HGpd;
+  GFace n q (Hq: q <= n) (ε: arity): G0 n.+1 -> G0 n;
+  GFaceCoh n q (Hq: q <= n) r (Hr: r <= q) (ε ω: arity) (X: G0 n.+2):
+    GFace n q Hq ε (GFace n.+1 r (Hr ↕ (↑ Hq)) ω X) =
+    GFace n r (Hr ↕ Hq) ω (GFace n.+1 q.+1 (⇑ Hq) ε X);
+  GFaceCoh2 n q (Hq: q <= n) r (Hr: r <= q) s (Hs: s <= r)
+    (ε ω θ: arity) (X: G0 n.+3):
+    f_equal (GFace n q Hq ε) (GFaceCoh n.+1 r (Hr ↕ (↑ Hq)) s Hs ω θ X)
+    • (GFaceCoh n q Hq s (Hs ↕ Hr) ε θ
+        (GFace n.+2 r.+1 (⇑ (Hr ↕ (↑ Hq))) ω X)
+    • f_equal (GFace n s (Hs ↕ (Hr ↕ Hq)) θ)
+        (GFaceCoh n.+1 q.+1 (⇑ Hq) r.+1 (⇑ Hr) ε ω X)) =
+    GFaceCoh n q Hq r Hr ε ω (GFace n.+2 s (↑ (↑ (Hs ↕ (Hr ↕ Hq)))) θ X)
+    • (f_equal (GFace n r (Hr ↕ Hq) ω)
+        (GFaceCoh n.+1 q.+1 (⇑ Hq) s (↑ (Hs ↕ Hr)) ε θ X)
+    • GFaceCoh n r (Hr ↕ Hq) s Hs ω θ (GFace n.+2 q.+2 (⇑ (⇑ Hq)) ε X))
+}.
+
+Arguments G0 {arity} _ _.
+Arguments GFace {arity} _ _ _ _ _.
+Arguments GFaceCoh {arity} _ _ _ _ _ _ _ _ _.
+Arguments GFaceCoh2 {arity} _ _ _ _ _ _ _ _ _ _ _ _.
+
+Definition AugmentedSemiSimplicialPresheafGpd := PresheafGpd hunit.
+Definition SemiCubicalPresheafGpd := PresheafGpd hbool.
+
+Section PresentationEq.
+Context (A: HSet).
+
+(** Equality of presentations
+
+    Over a fixed family of levels, pointwise identifications of the face
+    maps determine an equality of presentations when their squares commute
+    with the exchange paths. [GUIP] identifies the transported hexagon fields. *)
+
+Definition GFaceType (G: nat -> HGpd) :=
+  forall n q (Hq: q <= n) (ε: A), G (S n) -> G n.
+
+Definition GCohType {G: nat -> HGpd} (Fa: GFaceType G) :=
+  CohOf (Build_FaceStr A G Fa).
+
+Definition GCoh2Type {G: nat -> HGpd} {Fa: GFaceType G} (Ca: GCohType Fa) :=
+  Coh2Of Ca.
+
+(** The commuting square between two exchange laws over a pointwise
+    identification of their face families. *)
+
+Definition GSqType {G: nat -> HGpd} {Fa Fa': GFaceType G}
+  (Ca: GCohType Fa) (Ca': GCohType Fa')
+  (φ: forall n q (Hq: q <= n) (ε: A) x, Fa n q Hq ε x = Fa' n q Hq ε x): Type :=
+  forall n q (Hq: q <= n) r (Hr: r <= q) (ε ω: A) (X: G (S (S n))),
+     Ca n q Hq r Hr ε ω X
+     • (φ n r (Hr ↕ Hq) ω (Fa (S n) (S q) (⇑ Hq) ε X)
+        • f_equal (Fa' n r (Hr ↕ Hq) ω) (φ (S n) (S q) (⇑ Hq) ε X))
+     = (φ n q Hq ε (Fa (S n) r (Hr ↕ (↑ Hq)) ω X)
+        • f_equal (Fa' n q Hq ε) (φ (S n) r (Hr ↕ (↑ Hq)) ω X))
+       • Ca' n q Hq r Hr ε ω X.
+
+Lemma gpdEqHom {G: nat -> HGpd} (Fa Fa': GFaceType G)
+  (Ca: GCohType Fa) (Ca': GCohType Fa')
+  (Da: GCoh2Type Ca) (Da': GCoh2Type Ca')
+  (φ: forall n q (Hq: q <= n) (ε: A) x, Fa n q Hq ε x = Fa' n q Hq ε x)
+  (Hsq: GSqType Ca Ca' φ):
+  Build_PresheafGpd A G Fa Ca Da = Build_PresheafGpd A G Fa' Ca' Da'.
+Proof.
+  revert Ca' Da' Hsq.
+  refine (homInd5S (I1 := nat) (I2 := fun _ => nat) (I3 := fun n q => q <= n)
+            (I4 := fun _ _ _ => A) (I5 := fun n _ _ _ => G (S n))
+            (B := fun n _ _ _ _ => G n) Fa
+            (fun Fb φb => forall (Cb: GCohType Fb) (Db: GCoh2Type Cb),
+               GSqType Ca Cb φb ->
+               Build_PresheafGpd A G Fa Ca Da = Build_PresheafGpd A G Fb Cb Db)
+            _ Fa' φ).
+  intros Cb Db Hsq.
+  assert (e: Ca = Cb).
+  { apply functional_extensionality_dep; intro n.
+    apply functional_extensionality_dep; intro q.
+    apply spropFunext; intro Hq.
+    apply functional_extensionality_dep; intro r.
+    apply spropFunext; intro Hr.
+    apply functional_extensionality_dep; intro ε.
+    apply functional_extensionality_dep; intro ω.
+    apply functional_extensionality_dep; intro X.
+    now exact (Hsq n q Hq r Hr ε ω X • eq_trans_refl_l _). }
+  destruct e.
+  assert (e2: Da = Db).
+  { apply functional_extensionality_dep; intro n.
+    apply functional_extensionality_dep; intro q.
+    apply spropFunext; intro Hq.
+    apply functional_extensionality_dep; intro r.
+    apply spropFunext; intro Hr.
+    apply functional_extensionality_dep; intro s.
+    apply spropFunext; intro Hs.
+    apply functional_extensionality_dep; intro ε.
+    apply functional_extensionality_dep; intro ω.
+    apply functional_extensionality_dep; intro θ.
+    apply functional_extensionality_dep; intro X.
+    now exact ((G n).(GUIP)). }
+  now destruct e2.
+Qed.
+
+End PresentationEq.
